theories/Dot/hkdot/hkdot.v
@@ -28,8 +28,11 @@ Module Type HoSemJudgments
   (Import HST : HoSemTypes VS LWP L).
 
 (** Kinded, Indexed SubTyPing *)
+Notation sstpiK' i Γ T1 T2 K :=
+  (∀ ρ, sG⟦Γ⟧*ρ → ▷^i K ρ (envApply T1 ρ) (envApply T2 ρ))%I.
+
 Definition sstpiK `{dlangG Σ} {n} i Γ T1 T2 (K : sf_kind Σ n) : iProp Σ :=
-  ∀ ρ, sG⟦Γ⟧*ρ → ▷^i K ρ (envApply T1 ρ) (envApply T2 ρ).
+  |==> sstpiK' i Γ T1 T2 K.
 Arguments sstpiK : simpl never.
 Instance: Params (@sstpiK) 5 := {}.
 Notation "Γ s⊨ T1 <:[ i  ] T2 ∷ K" := (sstpiK i Γ T1 T2 K)
@@ -44,7 +47,7 @@ Notation "Γ s⊨ T ∷[ i  ] K" := (Γ s⊨ T <:[ i ] T ∷ K)
 
 (* Semantic SubKinding *)
 Definition sSkd `{dlangG Σ} {n} i Γ (K1 K2 : sf_kind Σ n) : iProp Σ :=
-  ∀ ρ, sG⟦Γ⟧*ρ → ∀ (T1 T2 : hoLtyO Σ n), ▷^i (K1 ρ T1 T2 → K2 ρ T1 T2).
+  |==> ∀ ρ, sG⟦Γ⟧*ρ → ∀ (T1 T2 : hoLtyO Σ n), ▷^i (K1 ρ T1 T2 → K2 ρ T1 T2).
 Arguments sSkd : simpl never.
 Instance: Params (@sSkd) 5 := {}.
 Notation "Γ s⊨ K1 <∷[ i  ] K2" := (sSkd i Γ K1 K2)
@@ -74,7 +77,7 @@ Section gen_lemmas.
     Γ s⊨ T1 <:[ i ] T2 ∷ K -∗
     S :: Γ s⊨ oShift T1 <:[ i ] oShift T2 ∷ kShift K.
   Proof.
-    iIntros "#HK %ρ /= #[Hg _]".
+    iIntros ">#HK !> %ρ /= #[Hg _]".
     by iApply (sf_kind_proper with "(HK Hg)").
   Qed.
 
@@ -92,7 +95,7 @@ Section gen_lemmas.
     Γ s⊨ K1 <∷[ i ] K2 -∗
     S :: Γ s⊨ kShift K1 <∷[ i ] kShift K2.
   Proof.
-    iIntros "#HK %ρ /= #[Hg _] *".
+    iIntros ">#HK !> %ρ /= #[Hg _] *".
     iApply ("HK" with "Hg").
   Qed.
 
@@ -101,7 +104,7 @@ Section gen_lemmas.
     S1 :: Γ s⊨ T <:[ i ] U ∷ K -∗
     S2 :: Γ s⊨ T <:[ i ] U ∷ K.
   Proof.
-    iIntros "#HsubS #HJ %ρ /= #[Hg HS]".
+    iIntros ">#HsubS >#HJ !> %ρ /= #[Hg HS]".
     iApply ("HJ" $! ρ with "[$Hg]").
     iApply ("HsubS" $! ρ with "[$Hg $HS] HS").
   Qed.
@@ -125,7 +128,7 @@ Section gen_lemmas.
     S1 :: Γ s⊨ K1 <∷[ i ] K2 -∗
     S2 :: Γ s⊨ K1 <∷[ i ] K2.
   Proof.
-    iIntros "#HsubS #HJ %ρ /= #[Hg HS] *".
+    iIntros ">#HsubS >#HJ !> %ρ /= #[Hg HS] *".
     iApply ("HJ" $! ρ with "[$Hg]").
     iApply ("HsubS" $! ρ with "[$Hg $HS] HS").
   Qed.
@@ -143,8 +146,8 @@ Section gen_lemmas.
       iIntros (v); [iIntros "[]" | iIntros "_ //"].
   Qed.
 
-  Lemma ksubtyping_equiv i Γ T1 T2 :
-    Γ s⊨ T1 <:[ i ] T2 ∷ sf_star ⊣⊢
+  Lemma ksubtyping_equiv' i Γ T1 T2 :
+    sstpiK' i Γ T1 T2 sf_star ⊣⊢
     ∀ ρ, sG⟦ Γ ⟧* ρ → ▷^i (oClose T1 ρ ⊆ oClose T2 ρ).
   Proof.
     iSplit.
@@ -155,16 +158,21 @@ Section gen_lemmas.
       iApply ("Hsub" with "Hg").
   Qed.
 
+  Lemma ksubtyping_equiv i Γ T1 T2 :
+    Γ s⊨ T1 <:[ i ] T2 ∷ sf_star ⊣⊢
+    |==> ∀ ρ, sG⟦ Γ ⟧* ρ → ▷^i (oClose T1 ρ ⊆ oClose T2 ρ).
+  Proof. rewrite /sstpiK; f_equiv. apply ksubtyping_equiv'. Qed.
+
   Lemma ksubtyping_spec ρ i Γ T1 T2 :
-    Γ s⊨ T1 <:[ i ] T2 ∷ sf_star -∗
+    sstpiK' i Γ T1 T2 sf_star -∗
     sG⟦ Γ ⟧* ρ -∗
     ▷^i (oClose T1 ρ ⊆ oClose T2 ρ).
   Proof.
-    rewrite ksubtyping_equiv; iIntros "Hsub Hg"; iApply ("Hsub" with "Hg").
+    rewrite ksubtyping_equiv'. iIntros "Hsub Hg"; iApply ("Hsub" with "Hg").
   Qed.
 
   Lemma ksubtyping_intro i Γ (T1 T2 : oltyO Σ 0) :
-    (∀ ρ, sG⟦ Γ ⟧* ρ →
+    (|==> ∀ ρ, sG⟦ Γ ⟧* ρ →
     ∀ v, ▷^i (oClose T1 ρ v → oClose T2 ρ v)) -∗
     Γ s⊨ T1 <:[ i ] T2 ∷ sf_star.
   Proof.
@@ -173,20 +181,20 @@ Section gen_lemmas.
   Qed.
 
   Lemma ksubtyping_intro_swap i Γ (T1 T2 : oltyO Σ 0) :
-    (∀ ρ, sG⟦ Γ ⟧* ρ →
+    (|==> ∀ ρ, sG⟦ Γ ⟧* ρ →
     ∀ v, ▷^i oClose T1 ρ v → ▷^i oClose T2 ρ v) -∗
     Γ s⊨ T1 <:[ i ] T2 ∷ sf_star.
   Proof using HswapProp.
-    rewrite -ksubtyping_intro; iIntros "#Hsub %ρ #Hg *".
+    rewrite -ksubtyping_intro; iIntros ">#Hsub !> %ρ #Hg *".
     iApply (impl_laterN with "(Hsub Hg)").
   Qed.
 
   Lemma kinding_intro Γ i (L T U : oltyO Σ 0) :
-    (∀ ρ, sG⟦ Γ ⟧* ρ →
+    (|==> ∀ ρ, sG⟦ Γ ⟧* ρ →
     ▷^i (oClose L ρ ⊆ oClose T ρ ⊆ oClose U ρ)) -∗
     Γ s⊨ T ∷[ i ] sf_kintv L U.
   Proof.
-    iIntros "#Hsub" (ρ); rewrite /= sr_kintv_refl /=. iApply "Hsub".
+    iIntros ">#Hsub !>" (ρ); rewrite /= sr_kintv_refl /=. iApply "Hsub".
   Qed.
 
   (** * Prefixes: K for Kinding, KStp for kinded subtyping, Skd for subkinding. *)
@@ -196,14 +204,14 @@ Section gen_lemmas.
   Lemma sK_Sing Γ (T : oltyO Σ 0) i :
     ⊢ Γ s⊨ T ∷[ i ] sf_sngl T.
   Proof.
-    rewrite -kinding_intro; iIntros "%ρ _". by rewrite -subtype_refl.
+    rewrite -kinding_intro; iIntros "!> %ρ _". by rewrite -subtype_refl.
   Qed.
 
   Lemma sKStp_Intv Γ (T1 T2 L U : oltyO Σ 0) i :
     Γ s⊨ T1 <:[i] T2 ∷ sf_kintv L U -∗
     Γ s⊨ T1 <:[i] T2 ∷ sf_kintv T1 T2.
   Proof.
-    iIntros "#Hs %ρ Hg"; iDestruct ("Hs" with "Hg") as "{Hs} (_ & #H & _)".
+    iIntros ">#Hs !> %ρ Hg"; iDestruct ("Hs" with "Hg") as "{Hs} (_ & #H & _)".
     rewrite /= /sr_kintv; iNext i. iDestruct "H" as "#$ {H}".
     by rewrite -!subtype_refl.
   Qed.
@@ -211,7 +219,7 @@ Section gen_lemmas.
   Lemma sK_Star Γ (T : oltyO Σ 0) i :
     ⊢ Γ s⊨ T ∷[ i ] sf_star.
   Proof.
-    rewrite -kinding_intro; iIntros "%ρ _ !>".
+    rewrite -kinding_intro; iIntros "!> %ρ _ !>".
     by iSplit; iIntros "%v /="; [iIntros "[]"|iIntros "_"].
   Qed.
 
@@ -221,7 +229,7 @@ Section gen_lemmas.
     Γ s⊨ K1 <∷[ i ] K2 -∗
     Γ s⊨ T1 <:[ i ] T2 ∷ K2.
   Proof.
-    iIntros "#H1 #Hsub %ρ #Hg". iApply ("Hsub" with "Hg (H1 Hg)").
+    iIntros ">#H1 >#Hsub !> %ρ #Hg". iApply ("Hsub" with "Hg (H1 Hg)").
   Qed.
 
   (** Kind subsumption (for kinding). *)
@@ -240,7 +248,7 @@ Section gen_lemmas.
     oLaterN i (oShift S) :: Γ s⊨ T1 <:[i] T2 ∷ K -∗
     Γ s⊨ oLam T1 <:[i] oLam T2 ∷ sf_kpi S K.
   Proof using HswapProp.
-    iIntros "#HTK %ρ #Hg * /=" (arg).
+    iIntros ">#HTK !> %ρ #Hg * /=" (arg).
     rewrite -impl_laterN.
     iIntros "Hs".
     iSpecialize ("HTK" $! (arg .: ρ) with "[$Hg $Hs]").
@@ -258,7 +266,7 @@ Section gen_lemmas.
     Γ s⊨ U1 <:[ i ] U2 ∷ sf_star -∗
     Γ s⊨ sf_kintv L1 U1 <∷[ i ] sf_kintv L2 U2.
   Proof.
-    iIntros "#HsubL #HsubU %ρ #Hg /=" (T1 T2).
+    iIntros ">#HsubL >#HsubU !> %ρ #Hg /=" (T1 T2).
     iPoseProof (ksubtyping_spec with "HsubL Hg") as "{HsubL} HsubL".
     iPoseProof (ksubtyping_spec with "HsubU Hg") as "{HsubU Hg} HsubU".
     iNext i; iIntros "#(HsubL1 & $ & HsubU1)"; iSplit.
@@ -271,7 +279,7 @@ Section gen_lemmas.
     oLaterN i (oShift S2) :: Γ s⊨ K1 <∷[ i ] K2 -∗
     Γ s⊨ sf_kpi S1 K1 <∷[ i ] sf_kpi S2 K2.
   Proof using HswapProp.
-    iIntros "#HsubS #HsubK %ρ #Hg /=".
+    iIntros ">#HsubS >#HsubK !> %ρ #Hg /=".
     iPoseProof (ksubtyping_spec with "HsubS Hg") as "{HsubS} HsubS".
     iAssert (∀ arg : vl, let ρ' := arg .: ρ in
             ▷^i (oClose S2 ρ arg → ∀ T1 T2 : hoLtyO Σ n,
@@ -290,14 +298,14 @@ Section gen_lemmas.
   prove them anyway, to show they hold regardless of extensions. *)
   Lemma sSkd_Refl {n} Γ i (K : sf_kind Σ n) :
     ⊢ Γ s⊨ K <∷[ i ] K.
-  Proof. iIntros "%ρ Hg * !> $". Qed.
+  Proof. iIntros "!> %ρ Hg * !> $". Qed.
 
   Lemma sSkd_Trans {n} Γ i (K1 K2 K3 : sf_kind Σ n) :
     Γ s⊨ K1 <∷[ i ] K2 -∗
     Γ s⊨ K2 <∷[ i ] K3 -∗
     Γ s⊨ K1 <∷[ i ] K3.
   Proof.
-    iIntros "#Hs1 #Hs2 %ρ #Hg *".
+    iIntros ">#Hs1 >#Hs2 !> %ρ #Hg *".
     iSpecialize ("Hs1" with "Hg"); iSpecialize ("Hs2" with "Hg"); iNext i.
     iIntros "{Hg} HK1". iApply ("Hs2" with "(Hs1 HK1)").
   Qed.
@@ -329,7 +337,7 @@ Section gen_lemmas.
     Γ s⊨ T2 <:[ i ] T3 ∷ K -∗
     Γ s⊨ T1 <:[ i ] T3 ∷ K.
   Proof.
-    iIntros "#Hs1 #Hs2 %ρ #Hg".
+    iIntros ">#Hs1 >#Hs2 !> %ρ #Hg".
     iApply (sf_kind_sub_trans with "(Hs1 Hg) (Hs2 Hg)").
   Qed.
 
@@ -338,17 +346,17 @@ Section gen_lemmas.
 
   Lemma sKStp_Top Γ (T : oltyO Σ 0) i :
     ⊢ Γ s⊨ T <:[ i ] ⊤ ∷ sf_star.
-  Proof. rewrite -ksubtyping_intro. iIntros "%ρ * _ * !> _ //". Qed.
+  Proof. rewrite -ksubtyping_intro. iIntros "!> %ρ * _ * !> _ //". Qed.
   Lemma sKStp_Bot Γ (T : oltyO Σ 0) i :
     ⊢ Γ s⊨ ⊥ <:[ i ] T ∷ sf_star.
-  Proof. rewrite -ksubtyping_intro; iIntros "%ρ * _ * !> []". Qed.
+  Proof. rewrite -ksubtyping_intro; iIntros "!> %ρ * _ * !> []". Qed.
 
   (* XXX <:-..-U *)
   Lemma sKStp_IntvU {Γ T1 T2 L U i} :
     Γ s⊨ T1 <:[i] T2 ∷ sf_kintv L U -∗
     Γ s⊨ T2 <:[i] U ∷ sf_star.
   Proof.
-    rewrite -ksubtyping_intro; iIntros "#HK * Hg *".
+    rewrite -ksubtyping_intro; iIntros ">#HK !> * Hg *".
     iDestruct ("HK" with "Hg") as "[_ [_ Hsub]]".
     iNext i; iApply "Hsub".
   Qed.
@@ -364,7 +372,7 @@ Section gen_lemmas.
     Γ s⊨ T1 <:[i] T2 ∷ sf_kintv L U -∗
     Γ s⊨ L <:[i] T1 ∷ sf_star.
   Proof.
-    rewrite -ksubtyping_intro; iIntros "#HK * Hg *".
+    rewrite -ksubtyping_intro; iIntros ">#HK !> * Hg *".
     iDestruct ("HK" with "Hg") as "[Hsub _]".
     iNext i; iApply "Hsub".
   Qed.
@@ -411,7 +419,7 @@ Section dot_types.
     oLaterN i T :: Γ s⊨p p : U, i -∗
     Γ s⊨p p.|[v/] : U.|[v/], i.
   Proof.
-    iIntros "#Hrepl #H" (ρ) "#Hg /=".
+    iIntros ">#Hrepl >#H !>" (ρ) "#Hg /=".
     iSpecialize ("Hrepl" with "Hg"); rewrite path_wp_pv_eq.
     rewrite hsubst_comp -subst_swap_base.
     iSpecialize ("H" $! (v.[ρ] .: ρ) with "[$Hg $Hrepl]").
@@ -426,7 +434,7 @@ Section dot_types.
     oLaterN i V :: Γ s⊨ T1 <:[ i ] T2 ∷ K -∗
     Γ s⊨ T1.|[v/] <:[ i ] T2.|[v/] ∷ K.|[v/].
   Proof.
-    iIntros "#Hrepl #H" (ρ) "#Hg /=".
+    iIntros ">#Hrepl >#H !>" (ρ) "#Hg /=".
     iSpecialize ("Hrepl" with "Hg"); rewrite path_wp_pv_eq -subst_swap_base.
     iSpecialize ("H" $! (v.[ρ] .: ρ) with "[$Hg $Hrepl]").
     iApply (sf_kind_proper with "H") => args w /=;
@@ -438,7 +446,7 @@ Section dot_types.
     Γ s⊨p p : S, i -∗
     Γ s⊨ oTApp T1 p <:[i] oTApp T2 p ∷ kpSubstOne p K.
   Proof.
-    iIntros "#HTK #Hp %ρ #Hg".
+    iIntros ">#HTK >#Hp !> %ρ #Hg".
     iApply (strong_path_wp_wand with "(Hp Hg)").
     iIntros (v Hal%alias_paths_pv_eq_1) "{Hp} #Hv".
     iApply (sf_kind_proper with "(HTK Hg Hv)") => args w /=;
@@ -457,8 +465,10 @@ Section dot_types.
     Γ s⊨p pv v : S, i -∗
     Γ s⊨ oTAppV T1 v <:[i] oTAppV T2 v ∷ K.|[v/].
   Proof.
-    rewrite -!oTApp_pv. iIntros "#HTK #Hv %ρ #Hg"; rewrite kpSubstOne_eq.
-    iApply (sKStp_App with "HTK Hv Hg").
+    rewrite -!oTApp_pv; iIntros "#HTK #Hv".
+    iPoseProof (sKStp_App with "HTK Hv") as ">Happ".
+    iIntros "!> %ρ #Hg"; rewrite kpSubstOne_eq.
+    iApply ("Happ" with "Hg").
   Qed.
 
   Lemma sK_AppV Γ {n} (K : sf_kind Σ n) {S T i v} :
@@ -496,7 +506,7 @@ Section dot_types.
   Lemma sstpiK_star_to_sstp Γ i T1 T2 :
     Γ s⊨ T1 <:[ i ] T2 ∷ sf_star ⊢ Γ s⊨ T1 , i <: T2 , i.
   Proof.
-    iIntros "#Hsub %ρ %v #Hg".
+    iIntros ">#Hsub !> %ρ %v #Hg".
     iDestruct (ksubtyping_spec with "Hsub Hg") as "{Hsub Hg} Hsub".
     rewrite -laterN_impl. iNext i. iApply ("Hsub" $! v).
   Qed.
@@ -505,7 +515,7 @@ Section dot_types.
     Γ s⊨ T1 <:[ i ] T2 ∷ sf_star ⊣⊢ Γ s⊨ T1 , i <: T2 , i.
   Proof using HswapProp.
     iSplit; first iApply sstpiK_star_to_sstp.
-    rewrite -ksubtyping_intro_swap /=. iIntros "#Hsub %ρ Hg *".
+    rewrite -ksubtyping_intro_swap /=. iIntros ">#Hsub !> %ρ Hg *".
     iApply ("Hsub" with "Hg").
   Qed.
 
@@ -518,7 +528,7 @@ Section dot_types.
     Γ s⊨ K1 <∷[ i ] K2 -∗
     Γ s⊨ oTMemK l K1 <:[ i ] oTMemK l K2 ∷ sf_star.
   Proof.
-    rewrite -ksubtyping_intro; iIntros "#HK %ρ Hg *".
+    rewrite -ksubtyping_intro; iIntros ">#HK !> %ρ Hg *".
     iSpecialize ("HK" with "Hg"); iNext i.
     iDestruct 1 as (d Hld) "Hφ"; iExists d; iFrame (Hld).
     iDestruct "Hφ" as (φ) "[Hlφ #HK1]"; iExists φ; iFrame "Hlφ".
@@ -528,7 +538,7 @@ Section dot_types.
   Lemma sKStp_TMem_AnyKind {n} Γ l (K : sf_kind Σ n) i :
     ⊢ Γ s⊨ oTMemK l K <:[ i ] oTMemAnyKind l ∷ sf_star.
   Proof.
-    rewrite -ksubtyping_intro; iIntros "%ρ #Hg * !>".
+    rewrite -ksubtyping_intro; iIntros "!> %ρ #Hg * !>".
     iDestruct 1 as (d Hl φ) "[Hl _]".
     iExists d; iFrame (Hl); iExists n, φ; iFrame "Hl".
   Qed.
@@ -549,8 +559,8 @@ Section dot_types.
     s ↝[ σ ] T -∗
     Γ s⊨ { l := dtysem σ s } : cTMemK l K.
   Proof.
-    rewrite sdtp_eq'; iIntros "#HTK"; iDestruct 1 as (φ Hγφ) "#Hγ".
-    iIntros (ρ Hpid) "Hg"; iExists (hoEnvD_inst (σ.|[ρ]) φ); iSplit.
+    rewrite sdtp_eq'; iIntros ">#HTK"; iDestruct 1 as (φ Hγφ) "#Hγ".
+    iIntros "!>" (ρ Hpid) "Hg"; iExists (hoEnvD_inst (σ.|[ρ]) φ); iSplit.
     by iApply (dm_to_type_intro with "Hγ").
     iApply (sf_kind_proper' with "(HTK Hg)") => args v /=.
     by rewrite -(Hγφ args ρ v).
@@ -560,7 +570,7 @@ Section dot_types.
     Γ s⊨p p : oTMemK l K, i -∗
     Γ s⊨ oSelN n p l ∷[i] K.
   Proof.
-    iIntros "#Hp %ρ Hg"; iSpecialize ("Hp" with "Hg"); iNext i.
+    iIntros ">#Hp !> %ρ Hg"; iSpecialize ("Hp" with "Hg"); iNext i.
     rewrite path_wp_eq.
     iDestruct "Hp" as (v Hal%alias_paths_pv_eq_1 d1 Hl1 ψ1) "[#Hl1 HK]".
     iApply (sfkind_respects with "[] HK"); iIntros (args w).
@@ -577,7 +587,7 @@ Section dot_types.
     Γ s⊨ T1 ∷[i] K -∗
     Γ s⊨ T1 <:[i] T2 ∷ K.
   Proof.
-    iIntros "#Hrepl #Hal #HK %ρ #Hg".
+    iIntros ">#Hrepl >#Hal >#HK !> %ρ #Hg".
     iSpecialize ("Hal" with "Hg"); iSpecialize ("HK" with "Hg"); iNext i.
     iDestruct "Hal" as %Hal%alias_paths_simpl.
     iApply (sf_kind_sub_internal_proper with "[] [] HK").
@@ -594,7 +604,7 @@ Section dot_types.
     Γ s⊨ T1 <:[i] T2 ∷ K1 -∗
     Γ s⊨ T1 <:[i] T2 ∷ K2.
   Proof.
-    iIntros "#Hal #HK %ρ #Hg".
+    iIntros ">#Hal >#HK !> %ρ #Hg".
     iSpecialize ("Hal" with "Hg"); iSpecialize ("HK" with "Hg"). iNext i.
     iDestruct "Hal" as %Hal%alias_paths_simpl.
     by iApply (Hrepl with "HK").
@@ -869,7 +879,7 @@ Section dot_experimental_kinds.
     that is, [oLam (oSing (pv (ids 0)))]. *)
   Proof.
     rewrite /sstpiK.
-    iIntros "/= #HT [#Hsub1 #Hsub2] %ρ #Hg"; iSpecialize ("HT" with "Hg");
+    iIntros "/= >#HT [>#Hsub1 >#Hsub2] !> %ρ #Hg"; iSpecialize ("HT" with "Hg");
       iSpecialize ("Hsub1" with "Hg"); iSpecialize ("Hsub2" with "Hg");
       iNext i.
     rewrite /sr_kintv/=.
