theories/Dot/lr/unary_lr.v
@@ -43,18 +43,18 @@ Section judgments.
 
   (** Expression typing *)
   Definition setp `{!dlangG Σ} e Γ τ : iProp Σ :=
-    ∀ ρ, sG⟦Γ⟧* ρ → sE⟦ τ ⟧ ρ (e.|[ρ]).
+    |==> ∀ ρ, sG⟦Γ⟧* ρ → sE⟦ τ ⟧ ρ (e.|[ρ]).
   Global Arguments setp : simpl never.
 
   (** Delayed subtyping. *)
   Definition sstpd `{!dlangG Σ} i Γ τ1 τ2 : iProp Σ :=
-    ∀ ρ,
+    |==> ∀ ρ,
       sG⟦Γ⟧*ρ → ▷^i (oClose τ1 ρ ⊆ oClose τ2 ρ).
   Global Arguments sstpd : simpl never.
 
   (** Multi-definition typing *)
   Definition sdstp `{!dlangG Σ} ds Γ (T : clty Σ) : iProp Σ :=
-    ⌜wf_ds ds⌝ ∧ ∀ ρ, ⌜path_includes (pv (ids 0)) ρ ds ⌝ → sG⟦Γ⟧* ρ → T ρ ds.|[ρ].
+    |==> ⌜wf_ds ds⌝ ∧ ∀ ρ, ⌜path_includes (pv (ids 0)) ρ ds ⌝ → sG⟦Γ⟧* ρ → T ρ ds.|[ρ].
   Global Arguments sdstp : simpl never.
 
   (** Definition typing *)
@@ -63,7 +63,7 @@ Section judgments.
 
   (** Path typing *)
   Definition sptp `{!dlangG Σ} p i Γ (T : oltyO Σ 0): iProp Σ :=
-    ∀ ρ, sG⟦Γ⟧* ρ →
+    |==> ∀ ρ, sG⟦Γ⟧* ρ →
       ▷^i path_wp p.|[ρ] (oClose T ρ).
   Global Arguments sptp : simpl never.
 End judgments.
@@ -84,15 +84,15 @@ Section JudgEqs.
 
   Lemma sstpd_eq_1 Γ T1 i T2 :
     Γ s⊨ T1 <:[i] T2 ⊣⊢
-    ∀ ρ, sG⟦Γ⟧* ρ → ∀ v, ▷^i (T1 vnil ρ v → T2 vnil ρ v).
+    |==> ∀ ρ, sG⟦Γ⟧* ρ → ∀ v, ▷^i (T1 vnil ρ v → T2 vnil ρ v).
   Proof.
-    rewrite /sstpd /subtype_lty; f_equiv => ρ.
+    rewrite /sstpd /subtype_lty; f_equiv; f_equiv => ρ.
     by rewrite laterN_forall.
   Qed.
 
   Lemma sstpd_eq Γ T1 i T2 :
     Γ s⊨ T1 <:[i] T2 ⊣⊢
-    ∀ ρ v, sG⟦Γ⟧* ρ → ▷^i (T1 vnil ρ v → T2 vnil ρ v).
+    |==> ∀ ρ v, sG⟦Γ⟧* ρ → ▷^i (T1 vnil ρ v → T2 vnil ρ v).
   Proof. rewrite sstpd_eq_1; properness. apply: forall_swap_impl. Qed.
 End JudgEqs.
 
@@ -130,7 +130,7 @@ Notation "T .sTp[ p /]" := (opSubst p T) (at level 65).
 
 (** Semantic definition of path replacement. *)
 Definition sem_ty_path_replI {Σ n} p q (T1 T2 : olty Σ n) : iProp Σ :=
-  ∀ args ρ v (H : alias_paths p.|[ρ] q.|[ρ]), T1 args ρ v ≡ T2 args ρ v.
+  |==> ∀ args ρ v (H : alias_paths p.|[ρ] q.|[ρ]), T1 args ρ v ≡ T2 args ρ v.
 Notation "T1 ~sTpI[ p := q  ]* T2" :=
   (sem_ty_path_replI p q T1 T2) (at level 70).
 
@@ -155,7 +155,7 @@ Section path_repl.
 
   Lemma sem_ty_path_repl_eq {n} {p q} {T1 T2 : olty Σ n} :
     T1 ~sTpP[ p := q ]* T2 → ⊢ T1 ~sTpI[ p := q ]* T2.
-  Proof. iIntros "%Heq !%". apply: Heq. Qed.
+  Proof. iIntros "%Heq !% /=". apply: Heq. Qed.
   (* The reverse does not hold. *)
 End path_repl.
 
@@ -317,21 +317,21 @@ Section judgment_definitions.
   Proof. by rewrite /path_includes path_wp_pure_pv_eq. Qed.
 
   Lemma idstp_eq Γ T ds : Γ ⊨ds ds : T ⊣⊢
-    ⌜wf_ds ds⌝ ∧ ∀ ρ, ⌜path_includes (pv (ids 0)) ρ ds ⌝ → G⟦Γ⟧ ρ → Ds⟦T⟧ ρ ds.|[ρ].
+    |==> ⌜wf_ds ds⌝ ∧ ∀ ρ, ⌜path_includes (pv (ids 0)) ρ ds ⌝ → G⟦Γ⟧ ρ → Ds⟦T⟧ ρ ds.|[ρ].
   Proof. reflexivity. Qed.
 
   Lemma ietp_eq Γ e T :
-    Γ ⊨ e : T ⊣⊢ ∀ ρ, G⟦Γ⟧ ρ → E⟦T⟧ ρ (e.|[ρ]).
+    Γ ⊨ e : T ⊣⊢ |==> ∀ ρ, G⟦Γ⟧ ρ → E⟦T⟧ ρ (e.|[ρ]).
   Proof. reflexivity. Qed.
 
   Lemma istpd_eq Γ T1 i T2 :
     Γ ⊨ T1 <:[i] T2 ⊣⊢
-    ∀ ρ v, G⟦Γ⟧ ρ → ▷^i (V⟦T1⟧ vnil ρ v → V⟦T2⟧ vnil ρ v).
+    |==> ∀ ρ v, G⟦Γ⟧ ρ → ▷^i (V⟦T1⟧ vnil ρ v → V⟦T2⟧ vnil ρ v).
   Proof. apply sstpd_eq. Qed.
 
   Lemma iptp_eq Γ p T i :
     Γ ⊨p p : T , i ⊣⊢
-    ∀ ρ, G⟦Γ⟧ ρ →
+    |==> ∀ ρ, G⟦Γ⟧ ρ →
       ▷^i path_wp (p.|[ρ]) (λ v, V⟦T⟧ vnil ρ v).
   Proof. reflexivity. Qed.
 End judgment_definitions.
@@ -437,7 +437,7 @@ Section misc_lemmas.
 
   Lemma sdtp_eq (Γ : sCtx Σ) (T : clty Σ) l d:
     Γ s⊨ { l := d } : T ⊣⊢
-      ∀ ρ, ⌜path_includes (pv (ids 0)) ρ [(l, d)]⌝ → sG⟦Γ⟧* ρ → T ρ [(l, d.|[ρ])].
+      |==> ∀ ρ, ⌜path_includes (pv (ids 0)) ρ [(l, d)]⌝ → sG⟦Γ⟧* ρ → T ρ [(l, d.|[ρ])].
   Proof.
     rewrite /sdtp /sdstp pure_True ?(left_id _ bi_and);
       by [> | exact: NoDup_singleton].
@@ -445,13 +445,13 @@ Section misc_lemmas.
 
   Lemma sdtp_eq' (Γ : sCtx Σ) (T : dlty Σ) l d:
     Γ s⊨ { l := d } : dty2clty l T ⊣⊢
-      ∀ ρ, ⌜path_includes (pv (ids 0)) ρ [(l, d)]⌝ → sG⟦Γ⟧* ρ → T ρ d.|[ρ].
+      |==> ∀ ρ, ⌜path_includes (pv (ids 0)) ρ [(l, d)]⌝ → sG⟦Γ⟧* ρ → T ρ d.|[ρ].
   Proof. by rewrite sdtp_eq; properness; last apply dty2clty_singleton. Qed.
 
   Lemma ipwp_terminates {p T i}:
     [] s⊨p p : T , i ⊢ ▷^i ⌜ terminates (path2tm p) ⌝.
   Proof.
-    iIntros "#H".
+    iIntros ">#H".
     iSpecialize ("H" $! ids with "[//]"); rewrite hsubst_id.
     iApply (path_wp_terminates with "H").
   Qed.
@@ -460,7 +460,7 @@ Section misc_lemmas.
   Lemma sT_Path {Γ τ p} :
     Γ s⊨p p : τ, 0 -∗ Γ s⊨ path2tm p : τ.
   Proof.
-    iIntros "#Hep %ρ #Hg /="; rewrite path2tm_subst.
+    iIntros ">#Hep !> %ρ #Hg /="; rewrite path2tm_subst.
     by iApply (path_wp_to_wp with "(Hep Hg)").
   Qed.
 End misc_lemmas.
