theories/Dot/examples/sem/small_sem_ex.v
@@ -62,7 +62,7 @@ Section small_ex.
       iApply suD_Sing; iApply suD_Val.
       iApply (suT_Sub (T1 := ipos)).
       unstamp_goal_tm.
-      by rewrite setp_value /ipos /pos; iIntros "%ρ _ /= !%"; naive_solver.
+      by rewrite setp_value /ipos /pos; iIntros "!> %ρ _ /= !%"; naive_solver.
       iApply sStp_Trans; first iApply sStp_Add_Later.
       iApply sStp_Trans; first iApply sStp_Add_Later.
       iApply sLater_Stp_Eq.
