theories/Dot/semtyp_lemmas/dsub_lr.v
@@ -35,52 +35,52 @@ Section DStpLemmas.
 
 
   Lemma sStp_Refl {Γ} T i : ⊢ Γ s⊨ T <:[i] T.
-  Proof. iIntros "%ρ _ !>"; by rewrite -subtype_refl. Qed.
+  Proof. iIntros "!> %ρ _ !>"; by rewrite -subtype_refl. Qed.
 
   Lemma sStp_Trans {Γ T1 T2 T3 i} :
     Γ s⊨ T1 <:[i] T2 -∗ Γ s⊨ T2 <:[i] T3 -∗ Γ s⊨ T1 <:[i] T3.
   Proof.
-    iIntros "#Hsub1 #Hsub2 %ρ #Hg *".
+    iIntros ">#Hsub1 >#Hsub2 !> %ρ #Hg *".
     iApply (subtype_trans with "(Hsub1 Hg) (Hsub2 Hg)").
   Qed.
 
   Lemma sStp_Top Γ T i:
     ⊢ Γ s⊨ T <:[i] oTop.
-  Proof. rewrite sstpd_eq_1. by iIntros "** !> ** /=". Qed.
+  Proof. rewrite sstpd_eq_1. by iIntros "!> ** !> **". Qed.
 
   Lemma sBot_Stp Γ T i:
     ⊢ Γ s⊨ oBot <:[i] T.
-  Proof. rewrite sstpd_eq_1. by iIntros "/= ** !> []". Qed.
+  Proof. rewrite sstpd_eq_1. by iIntros "!> /= ** !> []". Qed.
 
   Lemma sAnd1_Stp Γ T1 T2 i :
     ⊢ Γ s⊨ oAnd T1 T2 <:[i] T1.
-  Proof. rewrite sstpd_eq. by iIntros "/= %ρ %v _ !> [$ _]". Qed.
+  Proof. rewrite sstpd_eq. by iIntros "!> /= %ρ %v _ !> [$ _]". Qed.
   Lemma sAnd2_Stp Γ T1 T2 i :
     ⊢ Γ s⊨ oAnd T1 T2 <:[i] T2.
-  Proof. rewrite sstpd_eq. by iIntros "/= %ρ %v _ !> [_ $]". Qed.
+  Proof. rewrite sstpd_eq. by iIntros "!> /= %ρ %v _ !> [_ $]". Qed.
 
   Lemma sStp_And Γ T U1 U2 i:
     Γ s⊨ T <:[i] U1 -∗
     Γ s⊨ T <:[i] U2 -∗
     Γ s⊨ T <:[i] oAnd U1 U2.
   Proof.
-    rewrite !sstpd_eq; iIntros "#H1 #H2 %ρ %v #Hg".
+    rewrite !sstpd_eq; iIntros ">#H1 >#H2 !> %ρ %v #Hg".
     iSpecialize ("H1" $! ρ v with "Hg"); iSpecialize ("H2" $! ρ v with "Hg").
     iNext i; iIntros "#H".
     iSplit; [iApply "H1" | iApply "H2"]; iApply "H".
   Qed.
 
   Lemma sStp_Or1 Γ T1 T2 i: ⊢ Γ s⊨ T1 <:[i] oOr T1 T2.
-  Proof. rewrite sstpd_eq. by iIntros "/= %ρ %v _ !>"; eauto. Qed.
+  Proof. rewrite sstpd_eq. by iIntros "!> /= %ρ %v _ !>"; eauto. Qed.
   Lemma sStp_Or2 Γ T1 T2 i: ⊢ Γ s⊨ T2 <:[i] oOr T1 T2.
-  Proof. rewrite sstpd_eq. by iIntros "/= %ρ %v _ !>"; eauto. Qed.
+  Proof. rewrite sstpd_eq. by iIntros "!> /= %ρ %v _ !>"; eauto. Qed.
 
   Lemma sOr_Stp Γ T1 T2 U i:
     Γ s⊨ T1 <:[i] U -∗
     Γ s⊨ T2 <:[i] U -∗
     Γ s⊨ oOr T1 T2 <:[i] U.
   Proof.
-    rewrite !sstpd_eq; iIntros "/= #H1 #H2 * #Hg".
+    rewrite !sstpd_eq; iIntros ">#H1 >#H2 !> * #Hg".
     iSpecialize ("H1" $! ρ v with "Hg"); iSpecialize ("H2" $! ρ v with "Hg").
     iNext i; iIntros "#[HT | HT]"; [iApply "H1" | iApply "H2"]; iApply "HT".
   Qed.
@@ -88,7 +88,7 @@ Section DStpLemmas.
   Lemma sDistr_And_Or_Stp Γ {S T U i} : ⊢ Γ s⊨ oAnd (oOr S T) U <:[i] oOr (oAnd S U) (oAnd T U).
   Proof.
     rewrite sstpd_eq.
-    by iIntros "%ρ %v #Hg !> [[HS|HT] Hu] /="; [iLeft|iRight]; iFrame.
+    by iIntros "!> %ρ %v #Hg !> [[HS|HT] Hu] /="; [iLeft|iRight]; iFrame.
   Qed.
 
   (* XXX must we state the two separate halves? *)
@@ -99,7 +99,7 @@ Section DStpLemmas.
 
   Lemma sStp_Add_LaterN {Γ T i j}:
     ⊢ Γ s⊨ T <:[i] oLaterN j T.
-  Proof. rewrite sstpd_eq; iIntros "** !> $".  Qed.
+  Proof. rewrite sstpd_eq; iIntros "!> ** !> $".  Qed.
   Lemma sStp_Add_Later {Γ T i}:
     ⊢ Γ s⊨ T <:[i] oLater T.
   Proof. apply sStp_Add_LaterN. Qed.
@@ -108,7 +108,7 @@ Section DStpLemmas.
     Γ s⊨p p : oTMem l L U, i -∗
     Γ s⊨ L <:[i] oSel p l.
   Proof.
-    rewrite sstpd_eq; iIntros "#Hp %ρ %v Hg".
+    rewrite sstpd_eq; iIntros ">#Hp !> %ρ %v Hg".
     iSpecialize ("Hp" with "Hg"); iNext i; iIntros "#HL".
     iApply (path_wp_wand with "Hp"); iIntros (w).
     iApply (vl_sel_lb with "HL").
@@ -118,7 +118,7 @@ Section DStpLemmas.
     Γ s⊨p p : oTMem l L U, i -∗
     Γ s⊨ oSel p l <:[i] U.
   Proof.
-    rewrite sstpd_eq; iIntros "#Hp %ρ %v Hg".
+    rewrite sstpd_eq; iIntros ">#Hp !> %ρ %v Hg".
     iSpecialize ("Hp" with "Hg"); iNext i; iIntros "Hφ".
     iDestruct (path_wp_agree with "Hp Hφ") as (w Hw) "[Hp Hφ]".
     iApply (vl_sel_ub with "Hφ Hp").
@@ -133,7 +133,7 @@ Section DStpLemmas.
     oLaterN i T1 :: Γ s⊨ T1 <:[i] T2 -∗
     Γ s⊨ oMu T1 <:[i] oMu T2.
   Proof.
-    rewrite !sstpd_eq; iIntros "/= #Hstp %ρ %v Hg".
+    rewrite !sstpd_eq; iIntros ">#Hstp !> %ρ %v Hg".
     iApply mlaterN_impl; iIntros "#HT1".
     iApply ("Hstp" $! (v .: ρ) v with "[$Hg $HT1] [$HT1]").
   Qed.
@@ -177,7 +177,7 @@ Section DStpLemmas.
     Γ s⊨ T1 <:[i] T2 -∗
     Γ s⊨ oVMem l T1 <:[i] oVMem l T2.
   Proof.
-    iIntros "#Hsub %ρ Hg"; iSpecialize ("Hsub" with "Hg"); iNext i.
+    iIntros ">#Hsub !> %ρ Hg"; iSpecialize ("Hsub" with "Hg"); iNext i.
     iApply (oVMem_respects_sub with "Hsub").
   Qed.
 
@@ -186,7 +186,7 @@ Section DStpLemmas.
     Γ s⊨ U1 <:[i] U2 -∗
     Γ s⊨ oTMem l L1 U1 <:[i] oTMem l L2 U2.
   Proof.
-    iIntros "#HsubL #HsubU %ρ #Hg".
+    iIntros ">#HsubL >#HsubU !> %ρ #Hg".
     iSpecialize ("HsubL" with "Hg"); iSpecialize ("HsubU" with "Hg"); iNext i.
     iApply (oTMem_respects_sub with "HsubL HsubU").
   Qed.
@@ -196,7 +196,7 @@ Section DStpLemmas.
     oLaterN (i.+1) (oShift T2) :: Γ s⊨ oLater U1 <:[i] oLater U2 -∗
     Γ s⊨ oAll T1 U1 <:[i] oAll T2 U2.
   Proof.
-    rewrite !sstpd_delay_oLaterN_plus; iIntros "#HsubT #HsubU %ρ #Hg %v".
+    rewrite !sstpd_delay_oLaterN_plus; iIntros ">#HsubT >#HsubU !> %ρ #Hg %v".
     rewrite -!mlaterN_impl.
     iDestruct 1 as (t) "#[Heq #HT1]"; iExists t; iFrame "Heq".
     iIntros (w); iSpecialize ("HT1" $! w).
@@ -227,7 +227,7 @@ Section DStpLemmas.
     (*───────────────────────────────*)
     Γ s⊨ T1 <:[i] oLaterN j T2.
   Proof.
-    rewrite -sstpd_delay_oLaterN; iIntros "#Htyp %ρ Hg %v HvT1".
+    rewrite -sstpd_delay_oLaterN; iIntros ">#Htyp !> %ρ Hg %v HvT1".
     iEval rewrite /= -(path_wp_pv_eq _ (T2 _ _)) -laterN_plus.
     iApply ("Htyp" $! (v .: ρ) with "[$Hg $HvT1]").
   Qed.
@@ -249,7 +249,7 @@ Section DStpLemmas.
   Lemma sAnd_All_Stp_Distr Γ T U1 U2 i:
     ⊢ Γ s⊨ oAnd (oAll T U1) (oAll T U2) <:[i] oAll T (oAnd U1 U2).
   Proof.
-    iIntros "%ρ _ !> %v [#H1 #H2]".
+    iIntros "!> %ρ _ !> %v [#H1 #H2]".
     iDestruct "H1" as (t ?) "#H1"; iDestruct "H2" as (t' ->) "#H2"; simplify_eq.
     iExists t; iSplit; first done.
     iIntros (w) "#HT".
@@ -261,7 +261,7 @@ Section DStpLemmas.
   Lemma sAnd_Fld_Stp_Distr Γ l T1 T2 i:
     ⊢ Γ s⊨ oAnd (oVMem l T1) (oVMem l T2) <:[i] oVMem l (oAnd T1 T2).
   Proof.
-    iIntros "%ρ _ !> %v [#H1 H2]"; rewrite !oVMem_eq.
+    iIntros "!> %ρ _ !> %v [#H1 H2]"; rewrite !oVMem_eq.
     iDestruct "H1" as (pmem Hl) "#H1"; iDestruct "H2" as (pmem' Hl') "#H2".
     objLookupDet. iExists pmem; iFrame (Hl).
     by iApply (path_wp_and' with "H1 H2").
@@ -270,7 +270,7 @@ Section DStpLemmas.
   Lemma sAnd_Typ_Stp_Distr Γ l L U1 U2 i:
     ⊢ Γ s⊨ oAnd (oTMem l L U1) (oTMem l L U2) <:[i] oTMem l L (oAnd U1 U2).
   Proof.
-    iIntros "%ρ _ !> %v [H1 H2]"; rewrite !oTMem_eq /dot_intv_type_pred.
+    iIntros "!> %ρ _ !> %v [H1 H2]"; rewrite !oTMem_eq /dot_intv_type_pred.
     iDestruct "H1" as (ψ d Hl) "[Hdψ1 [HLψ1 HψU1]]".
     iDestruct "H2" as (ψ' d' Hl') "[Hdψ2 [_ HψU2]]". objLookupDet.
     iExists ψ, d. iFrame (Hl) "HLψ1". iSplit; first done.
@@ -283,7 +283,7 @@ Section DStpLemmas.
   Lemma sOr_Fld_Stp_Distr Γ l T1 T2 i:
     ⊢ Γ s⊨ oVMem l (oOr T1 T2) <:[i] oOr (oVMem l T1) (oVMem l T2).
   Proof.
-    iIntros "%ρ _ !> %v". rewrite !oVMem_eq.
+    iIntros "!> %ρ _ !> %v". rewrite !oVMem_eq.
     iDestruct 1 as (pmem Hl) "Hp". rewrite path_wp_eq.
     iDestruct "Hp" as (w Hpw) "[H|H]"; [iLeft|iRight].
     all: by rewrite oVMem_eq; iExists (pmem); iFrame (Hl);
@@ -295,7 +295,7 @@ Section DStpLemmas.
     Γ s⊨p p : oLater T, i -∗
     Γ s⊨p p : T, i.+1.
   Proof.
-    iIntros "#HpT %ρ #Hg"; rewrite -later_laterN laterN_later.
+    iIntros ">#HpT !> %ρ #Hg"; rewrite -later_laterN laterN_later.
     iSpecialize ("HpT" with "Hg"); iNext i.
     iApply (path_wp_later_swap with "HpT").
   Qed.
